

$$\begin{aligned}
 1. a) \lim_{n \rightarrow \infty} \frac{(n^2+1)^{10}}{n^{20}} &= \lim_{n \rightarrow \infty} \frac{\frac{d}{dn} (n^2+1)^{10}}{\frac{d}{dn} (n^{20})} \\
 &= \lim_{n \rightarrow \infty} \frac{(2n)(10)(n^2+1)^9}{20n^{19}} \\
 &= \lim_{n \rightarrow \infty} \frac{(n^2+1)^9}{n^{18}} \\
 &= \lim_{n \rightarrow \infty} \frac{\frac{d}{dn} ((n^2+1)^9)}{\frac{d}{dn} (n^{18})} \\
 &= \lim_{n \rightarrow \infty} \frac{2n(9)(n^2+1)^8}{18n^{17}} \\
 &= \lim_{n \rightarrow \infty} \frac{(n^2+1)^8}{n^{16}} \\
 &= \lim_{n \rightarrow \infty} \frac{\frac{d}{dn} ((n^2+1)^8)}{\frac{d}{dn} (n^{16})} \\
 &= \lim_{n \rightarrow \infty} \frac{2n(8)(n^2+1)^7}{16n^{15}} \\
 &= \lim_{n \rightarrow \infty} \frac{(n^2+1)^7}{n^{14}} \\
 &= \lim_{n \rightarrow \infty} \frac{2n(7)(n^2+1)^6}{14n^{13}} \\
 &= \lim_{n \rightarrow \infty} \frac{(n^2+1)^6}{n^{12}} \\
 &= \lim_{n \rightarrow \infty} \frac{2n(6)(n^2+1)^5}{12n^{11}} \\
 &= \lim_{n \rightarrow \infty} \frac{(n^2+1)^5}{n^{10}} \\
 &= \lim_{n \rightarrow \infty} \frac{2n(5)(n^2+1)^4}{10n^9} \\
 &= \lim_{n \rightarrow \infty} \frac{(n^2+1)^4}{n^8} \\
 &= \lim_{n \rightarrow \infty} \frac{2n(4)(n^2+1)^3}{8n^7} \\
 &= \lim_{n \rightarrow \infty} \frac{(n^2+1)^3}{n^6} \\
 &= \lim_{n \rightarrow \infty} \frac{2n(3)(n^2+1)^2}{6n^5}
 \end{aligned}$$

$$\begin{aligned} &= \lim_{n \rightarrow \infty} \frac{\sqrt[4]{(n^2+1)^2}}{\sqrt[4]{n^4}} \\ &= \lim_{n \rightarrow \infty} \frac{4n(n^2+1)}{4n^3} \\ &= \lim_{n \rightarrow \infty} \frac{n^2+1}{n^2} \\ &= \lim_{n \rightarrow \infty} \frac{2n}{2n} \\ &= 1 \end{aligned}$$

Due to the limit being a positive constant,  $(n^2+1)^{1/2} \in \Theta(n^2)$

$$\begin{aligned}
 b) \lim_{n \rightarrow \infty} \frac{\sqrt{10n^2 + 7n + 3}}{n} &= \lim_{n \rightarrow \infty} \frac{\sqrt{10|n|} + \sqrt{7n+3}}{n} \quad 0 \\
 &= \lim_{n \rightarrow \infty} \frac{\sqrt{10}|n|}{n} \\
 &= \pm \sqrt{10}
 \end{aligned}$$

Due to the limit being two constants,  $\sqrt{10n^2 + 7n + 3} \in \Theta(n)$

$$\begin{aligned}
 c) \lim_{n \rightarrow \infty} \frac{2n \lg(n+2)^2 + (n+2)^2 \lg \frac{n}{2}}{n^2 \lg n} &= \lim_{n \rightarrow \infty} \frac{4n \lg(n+2) + (n+2)^2 \lg n - \lg 2}{n^2 \lg n} \quad 0 \\
 &= \lim_{n \rightarrow \infty} \frac{4n \lg(n+2)}{n^2 \lg n} + \frac{(n+2)^2 \lg n}{n^2 \lg n} - \frac{\lg 2}{n^2 \lg n} \\
 &= \lim_{n \rightarrow \infty} \frac{(n^2 + 4n + 4) \lg n}{n^2 \lg n} \\
 &= \lim_{n \rightarrow \infty} \frac{n^2}{n^2} + \frac{4n}{n^2} + \frac{4}{n^2} \\
 &= 1
 \end{aligned}$$

Due to the limit being a positive constant,  $2n \lg(n+2)^2 + (n+2)^2 \lg \frac{n}{2} \in \Theta(n^2 \lg n)$

$$\begin{aligned}
 d) \lim_{n \rightarrow \infty} \frac{2^{n+1} + 3^{n-1}}{2^n + 3^n} &= \lim_{n \rightarrow \infty} \frac{2(2^n) + \frac{1}{3}(3^n)}{2^n + 3^n} \\
 &= \lim_{n \rightarrow \infty} \frac{3^n \left( 2 \left( \frac{2}{3} \right)^n + \frac{1}{3} \right)}{2^n + 3^n} \\
 &= \lim_{n \rightarrow \infty} \frac{3^n \left( 2 \left( \frac{2}{3} \right)^n + \frac{1}{3} \right)}{3^n \left( \left( \frac{2}{3} \right)^n + 1 \right)} \\
 &= \frac{2(0) + \frac{1}{3}}{0 + 1} \\
 &= \frac{1/3}{1} \\
 &= 1/3
 \end{aligned}$$

Due to the limit being a positive constant,  $2^{n+1} + 3^{n-1} \in \Theta(2^n + 3^n)$

$$e) \lim_{n \rightarrow \infty} \frac{\lfloor \log_2 n \rfloor}{\log_2 n} = \lfloor 1 \rfloor = 1$$

Due to the limit being a positive constant,  $\lfloor \log_2 n \rfloor \in \Theta(\log_2 n)$

$$2. \lim_{n \rightarrow \infty} \frac{(n-2)!}{(n-2)!} = \lim_{n \rightarrow \infty} \frac{(n-2) \times (n-3) \times \dots \times 1}{(n-2) \times (n-3) \times \dots \times 1} = 1$$

$\therefore 1 > 0 \rightarrow (n-2)! \in \Theta((n-2)!)$

$$\begin{aligned} \lim_{n \rightarrow \infty} \frac{5 \lg(n+100)^{10}}{\lg n} &= 5 \lim_{n \rightarrow \infty} \frac{10 \lg(n+100)}{\lg n} \\ &= 50 \lim_{n \rightarrow \infty} \frac{\frac{d}{dn}(\lg(n+100))}{\frac{d}{dn}(\lg n)} \\ &= 50 \lim_{n \rightarrow \infty} \frac{1}{\frac{(n+100) \ln 10}{1}} \\ &= 50 \lim_{n \rightarrow \infty} \frac{n \ln 10}{(n+100) \ln 10} \\ &= 50 \lim_{n \rightarrow \infty} \frac{n}{n+100} \\ &= 50 \lim_{n \rightarrow \infty} \frac{\frac{d}{dn}(n)}{\frac{d}{dn}(n+100)} \\ &= 50 \lim_{n \rightarrow \infty} \frac{1}{1} \\ &= 50 \end{aligned}$$

Due to the limit being a positive constant,  $5 \lg(n+100)^{10} \in \Theta(\lg n)$

$$\lim_{n \rightarrow \infty} \frac{2^{2n}}{2^n} = \lim_{n \rightarrow \infty} \frac{4(2^n)}{2^n} = 4$$

Due to the limit being a positive constant,  $2^{2n} \in \Theta(2^n)$

$$\begin{aligned} \lim_{n \rightarrow \infty} \frac{0.001n^4 + 3n^3 + 1}{n^4} &= \lim_{n \rightarrow \infty} \frac{0.001n^4}{n^4} + \frac{3n^3}{n^4} + \frac{1}{n^4} \\ &= \lim_{n \rightarrow \infty} 0.001 + 0 + 0 \\ &= 0.001 \end{aligned}$$

$$\lim_{n \rightarrow \infty} \frac{\ln^2(n)}{\ln^2(n)} = 1$$

Due to the limit being a positive constant,  $\ln^2(n) \in \Theta(\ln^2(n))$

$$\lim_{n \rightarrow \infty} \frac{\sqrt[3]{n}}{\sqrt[3]{n}} = 1$$

Due to the limit being a positive constant,  $\sqrt[3]{n} \in \Theta(\sqrt[3]{n})$

$$\lim_{n \rightarrow \infty} \frac{3^n}{3^n} = 1$$

Due to the limit being a positive constant,  $3^n \in \Theta(3^n)$

Order of Growth

Lowest  $\rightarrow$

$\leftarrow$  Highest

$5 \lg(n+100)^{10}, \sqrt[3]{n}, \ln^2(n), 0.001n^4 + 3n^3 + 1, 2^n, 3^n, (n-2)!$

$$\begin{aligned} 3. a) \sum_{i=1}^{500} 2^{i-1} &= \frac{500}{2} (1 + 999) \\ &= 250(1000) \\ &= 250000 \end{aligned}$$

$$b) \sum_{i=0}^{10} 2^i = 2^{10+1} - 1 = 2^{11} - 1 = 2047$$

$$c) \sum_{i=3}^{n+1} 1 = (n+1) - 3 + 1 = n - 1$$

$$d) \sum_{i=3}^{n+1} i = \frac{(n+1)(n+2)}{2} = \frac{n^2 + 3n + 2}{2}$$

$$\begin{aligned} e) \sum_{i=0}^{n-1} i(i+1) &= \frac{(n-1)(n)(2n-1)}{6} + \frac{(n-1)(n)}{2} \\ &= \frac{(n^2 - n)(2n-1)}{6} + \frac{n^2 - n}{2} \end{aligned}$$

$$= \frac{2n^3 - 3n^2 + n}{6} + \frac{n^2 - n}{2}$$

$$\begin{aligned}
 f) \sum_{j=1}^n 3^{j+1} &= \sum_{j=1}^n 3^j + 3 \sum_{j=1}^n 1 \\
 &= \frac{3^{n+1} - 1}{3 - 1} + 3(n - 1 + 1) \\
 &= \frac{3^{n+1} - 1}{2} + 3n
 \end{aligned}$$

$$\begin{aligned}
 g) \sum_{i=1}^n \sum_{j=1}^n ij &= \sum_{i=1}^n i \times \sum_{j=1}^n j \\
 &= \frac{n^2 + n}{2} \times \frac{n^2 + n}{2} = \left( \frac{n^2 + n}{2} \right)^2
 \end{aligned}$$

$$\begin{aligned}
 h) \sum_{i=1}^n \frac{1}{i(i+1)} &= \sum_{i=1}^n \frac{1}{i} - \sum_{i=1}^n \frac{1}{i+1} \\
 &= 1 + \ln(n) + \gamma
 \end{aligned}$$

$\gamma = 0.5772$

$$\begin{aligned}
 4. a) \sum_{i=0}^{n-1} (i^2 + 1)^2 &= \sum_{i=0}^{n-1} (i^4 + 2i^2 + 1) = \sum_{i=0}^{n-1} i^4 + 2 \sum_{i=0}^{n-1} i^2 + \sum_{i=0}^{n-1} 1 \\
 &= \frac{1}{5} (n-1)^5 + \frac{2}{3} (n-1)^3 + (n-1 - 0 + 1) \\
 &= \frac{1}{5} (n-1)^5 + \frac{2}{3} (n-1)^3 + n \\
 \lim_{n \rightarrow \infty} \frac{\frac{1}{5} (n-1)^5 + \frac{2}{3} (n-1)^3 + n}{n^5} &= \lim_{n \rightarrow \infty} \frac{\frac{d}{dn} \left( \frac{1}{5} (n-1)^5 + \frac{2}{3} (n-1)^3 + n \right)}{\frac{d}{dn} (n^5)} \\
 &= \lim_{n \rightarrow \infty} \frac{\frac{1}{5} (n-1)^4 + 2(n-1)^2 + 1}{5n^4} \\
 &= \lim_{n \rightarrow \infty} \frac{\frac{d}{dn} \left( \frac{1}{5} (n-1)^4 + 2(n-1)^2 + 1 \right)}{\frac{d}{dn} (5n^4)} \\
 &= \lim_{n \rightarrow \infty} \frac{\frac{1}{5} (3(n-1)^2 + 1)}{15n^3} \\
 &= \lim_{n \rightarrow \infty} \frac{n-1}{5n}
 \end{aligned}$$

$$= \frac{1}{5} \lim_{n \rightarrow \infty} \frac{\frac{d}{dn}(n-1)}{\frac{d}{dn}(n)} \\ = \frac{1}{5} \lim_{n \rightarrow \infty} 1 = 1/5$$

Due to the limit being a positive constant,

$$\sum_{i=0}^{n-1} (i^2 + 1)^2 \in \Theta(n^5)$$

$$b) \sum_{i=2}^{n-1} \lg i^2 = \sum_{i=2}^{n-1} \lg i \times \sum_{i=2}^{n-1} i = \lg 1$$

$$= (n-1) \lg(n-1) \times \frac{(n-1)(n)}{2} = \frac{n(n-1)^2 \lg(n-1)}{2} \\ = \frac{1}{2} \lim_{n \rightarrow \infty} \frac{(n^3 - 2n^2 + 2n) \lg(n-1)}{n^3 \lg n} = \lim_{n \rightarrow \infty} \frac{(n^3 - 2n^2 + 2n)}{n^3} \times \frac{\lg(n-1)}{\lg n} \\ = \lim_{n \rightarrow \infty} \frac{n^3}{n^3} - \frac{2}{n} + \frac{2}{n^2} \times \frac{\lg(n-1)}{\lg n} \\ = \lim_{n \rightarrow \infty} 1 \times \frac{\lg(n-1)}{\lg n} \\ = \lim_{n \rightarrow \infty} \frac{\frac{d}{dn}(\lg(n-1))}{\frac{d}{dn}(\lg n)} \\ = \lim_{n \rightarrow \infty} \frac{1/(n-1) \ln(10)}{1/n \ln(10)} \\ = \lim_{n \rightarrow \infty} \frac{n \ln(10)}{(n-1) \ln(10)} \\ = \lim_{n \rightarrow \infty} \frac{\frac{d}{dn}(n)}{\frac{d}{dn}(n-1)} \\ = \lim_{n \rightarrow \infty} \frac{1}{1} = 1$$

Due to the limit being a positive constant,

$$\sum_{i=2}^{n-1} \lg i^2 \in \Theta(n^3 \lg n)$$

$$\begin{aligned}
 c) \sum_{i=1}^n (i+1)2^{i-1} &= \left( \sum_{i=1}^n i + \sum_{i=1}^n 1 \right) \times \left( \sum_{i=1}^n 2^i - 1 \right) \times \frac{1}{2} \sum_{i=1}^n 1 \\
 &= \left( \frac{n(n+1)}{2} + n \right) \times \left( \frac{2^{n+1}-1}{2-1} - 1 \right) \times \frac{n}{2} \\
 &= \left( \frac{n^2+3n}{2} \right) \times (2^{n+1}-2) \times \frac{n}{2} \\
 &= \left( \frac{n^2+3n}{2} \times 2^n \times \frac{n}{2} \right) \\
 &= \frac{n^2(n+3)2^n}{4}
 \end{aligned}$$

$$\begin{aligned}
 \lim_{n \rightarrow \infty} \frac{\frac{1}{4} n^2(n+3)(2^n)}{n^3 2^n} &= \frac{1}{4} \lim_{n \rightarrow \infty} \frac{2^n (n^3 + 3n^2)}{n^3 2^n} \\
 &= \frac{1}{4} \lim_{n \rightarrow \infty} \frac{n^3 + 3n^2}{n^3} \\
 &= \frac{1}{4} \lim_{n \rightarrow \infty} \frac{n^3}{n^3} + \frac{3n^2}{n^3} \\
 &= \frac{1}{4}
 \end{aligned}$$

Due to the limit being a positive constant,  
 $\frac{1}{4} n^2(n+3)2^n \in \Theta(n^3 2^n)$

$$\begin{aligned}
 d) \sum_{i=0}^{n-1} \sum_{j=0}^{i-1} (i+j) &= \sum_{i=0}^{n-1} \left( \sum_{j=0}^{i-1} i + \sum_{j=0}^{i-1} j \right) \quad \leftarrow \text{constant here} \\
 &= \sum_{i=0}^{n-1} i \left( \sum_{j=0}^{i-1} 1 + \sum_{j=0}^{i-1} j \right) \\
 &= \sum_{i=0}^{n-1} i \left( i-1+1 + \frac{(i-1)i}{2} \right) \\
 &= \sum_{i=0}^{n-1} i \left( i + \frac{1}{2} i^2 - \frac{i}{2} \right) \\
 &= \frac{1}{2} \sum_{i=0}^{n-1} i^2 + i^3
 \end{aligned}$$



Pg 9 of 12

$$= \frac{1}{2} \left( \sum_{i=0}^{n-1} i^2 + \sum_{i=0}^{n-1} i^3 \right)$$

$$= \frac{1}{2} \left( \frac{(n-1)n(2n-1)}{6} + \frac{1}{4} (n-1)^4 \right)$$

$$= \frac{1}{4} \left( \frac{2n^3 - 3n^2 + n}{3} + \frac{(n-1)^4}{2} \right)$$

$$= \frac{1}{4} \lim_{n \rightarrow \infty} \frac{\frac{2n^3 - 3n^2 + n}{3} + \frac{(n-1)^4}{2}}{\frac{1}{n^4}}$$

$$= \frac{1}{4} \lim_{n \rightarrow \infty} \frac{\frac{1}{3}(6n^2 - 6n + 1) + 4(n-1)^3}{\frac{1}{n^4}(4n^3)}$$

$$= \frac{1}{4} \lim_{n \rightarrow \infty} \frac{\frac{1}{3}(12n - 6) + 12(n-1)^2}{12n^2}$$

$$= \frac{1}{4} \lim_{n \rightarrow \infty} \frac{\frac{1}{3}(2n - 1) + 2(n-1)^2}{\frac{1}{n^4}(6n^2)}$$

$$\rightarrow = \frac{1}{4} \lim_{n \rightarrow \infty} \frac{2 + 4n - 4}{12n}$$

$$= \frac{1}{4} \lim_{n \rightarrow \infty} \frac{2n - 1}{6n}$$

$$= \frac{1}{4} \lim_{n \rightarrow \infty} \frac{n}{3n} = \frac{1}{12}$$

$$= \frac{1}{4} \left( \frac{1}{3} \right)$$

$$= \frac{1}{12}$$

Due to the limit being a positive constant,

$$\frac{1}{4} \left( \frac{2n^3 - 3n^2 + n}{3} + \frac{(n-1)^4}{2} \right) \in \Theta(n^4)$$

So Formula #1:

$$\textcircled{1} \frac{\sum_{i=1}^n (x_i - \bar{x})^2}{n-1}$$

$$\textcircled{2} \frac{\sum_{i=1}^n x_i}{n}$$

$$\textcircled{2} \begin{cases} M(n) = 0 \\ D(n) = 1 \\ S(n) = 0 \\ A(n) = n-1 \end{cases}$$

$$\textcircled{1} \begin{cases} M(n) = n-1 \\ D(n) = 1(n-1) + 1 \\ S(n) = n-1 + 1 \\ A(n) = (n-1)(n-1) \end{cases}$$

The total operations for this formula are  $M(n) = n-1$ ,  $D(n) = n$ ,  $S = n$ ,  $A(n) = (n-1)^2$

Formula #2:

$$\sum_{i=1}^n x_i^2 - \left( \sum_{i=1}^n x_i \right)^2$$

$$\frac{\sum_{i=1}^n x_i^2 - \left( \sum_{i=1}^n x_i \right)^2}{n-1}$$

$$\text{Subst} \rightarrow \begin{cases} M(n) = 1 \\ D(n) = 1 \\ S(n) = 0 \\ A(n) = n-1 \end{cases}$$

entire formula

$$\begin{cases} M(n) = 2(n-1) \\ D(n) = n-1 + 1 \\ S(n) = n-1 + 1 \\ A(n) = (n-1)(n-1) \end{cases}$$

The total operations for this formula is  $M(n) = 2n-2$ ,  $D(n) = n$ ,  $S(n) = n$ ,  $A(n) = (n-1)^2$

6. a) This algorithm will sort an array numbers from greatest on the left to lowest on the right.

b) The basic operation is the if  $A[j] > A[i]$

$$\begin{aligned} c) \sum_{i=0}^{n-2} \sum_{j=i+1}^{n-1} 1 &= \sum_{i=0}^{n-2} (n-1-0+1) \\ &= \sum_{i=0}^{n-2} n \\ &= n \sum_{i=0}^{n-2} 1 = n(n-1-0+1) = n(n) = n^2 \end{aligned}$$

Thus, the basic operation is executed  $n^2$  times

$$d) \lim_{n \rightarrow \infty} \frac{n^2}{n^2} = 1$$

Due to the limit being a positive constant,  
 $n^2 \in \Theta(n^2)$

The efficiency class is  $n^2$ .

$$7. a) A(n) = 3A(n-1) \quad A(n-1) = 3A(n-2)$$

$$A(n) = 3^2 A(n-2) \quad A(n-2) = 3A(n-3)$$

$$A(n) = 3^3 A(n-3)$$

$$A(n) = 3^i A(n-i) \quad \text{Let } i = n-1$$

$$A(n) = 3^{n-1} A(n-(n-1))$$

$$A(n) = \frac{4}{3}(3^n) \quad \text{The solution to this recurrence equation is } A(n) = 3^n \left(\frac{4}{3}\right)$$

$$b) A(n) = A(n-1) + 5 \quad A(n-1) = A(n-2) + 5$$

$$A(n) = A(n-2) + 10 \quad A(n-2) = A(n-3) + 5$$

$$A(n) = A(n-3) + 15$$

$$A(n) = A(n-i) + 5i \quad \text{Let } i = n-1$$

$$A(n) = A(n-(n-1)) + 5(n-1)$$

$$A(n) = 5n - 5$$

The solution to this recurrence equation is  $A(n) = 5n - 5$

$$\begin{aligned}
 c) \quad A(n) &= A(n-1) + n & A(n-1) &= A(n-2) + n \\
 A(n) &= A(n-2) + 2n & A(n-2) &= A(n-3) + n \\
 A(n) &= A(n-3) + 3n \\
 A(n) &= A(n-i) + i(n) & \text{Let } i &= n \\
 A(n) &= A(n-n) + n^2 \\
 A(n) &= n^2
 \end{aligned}$$

The solution to this recurrence equation is  $A(n) = n^2$

$$\begin{aligned}
 d) \quad A(n) &= A(n/5) + 1 & A(5^0) &= 1 \\
 A(5^k) &= A(5^{k-1}) + 1 & A(5^{k-1}) &= A(5^{k-2}) + 1 \\
 A(5^k) &= A(5^{k-2}) + 2 & A(5^{k-2}) &= A(5^{k-3}) + 1 \\
 A(5^k) &= A(5^{k-3}) + 3 \\
 A(5^k) &= A(5^{k-i}) + i & i &= k \\
 A(5^k) &= A(5^{k-k}) + k \\
 A(5^k) &= k \\
 k &= \log_5 n
 \end{aligned}$$

The solution to this recurrence equation is  $A(n) = \log_5 n$

8. a) This algorithm computes the sum of the squared for all the numbers starting at 1 and leading up to  $n$ .

b) The basic operation is the multiplication in the recursive call.

$$\begin{aligned}
 c) \quad M(n) &= M(n-1) + 1 & M(1) &= 1 \\
 M(n) &= M(n-2) + 2 & M(n-1) &= M(n-2) + 1 \\
 M(n) &= M(n-i) + i & i &= n-1 \\
 M(n) &= M(n-n+1) + n-1 \\
 M(n) &= n-1
 \end{aligned}$$

The basic operation will get called  $n-1$  times for all  $n \geq 1$ .

$$\begin{aligned}
 d) \quad \lim_{n \rightarrow \infty} \frac{n-1}{n} &= \lim_{n \rightarrow \infty} \frac{n}{n} - \frac{1}{n} \\
 &= 1
 \end{aligned}$$

The efficiency class would be  $\Theta(n)$  where  $n-1 \in \Theta(n)$

Let  $n=4$ 

9. a)  $Q(n) = Q(n-1) + 2n - 1$

$Q(4) = Q(3) + 7 = 16$

$Q(3) = Q(2) + 5 = 9$

$Q(2) = Q(1) + 3 = 4$

This algorithm will compute the sum of all odd integers up to  $n$ .

b)  $M(n) = M(n-1) + 1$

$M(n-1) = M(n-2) + 1$

$M(1) = 0$

$M(n) = M(n-2) + 2$

$M(n-2) = M(n-3) + 1$

$M(n) = M(n-3) + 3$

$M(n) = M(n-i) + i$

$i = n-1$

$M(n) = M(n-n+1) + n-1$

$M(n) = n-1$

There are  $n-1$  multiplications made.

c)  $A(n) = A(n-1) + 2(1)$

$A(n-1) = A(n-2) + 2$

$A(1) = 0$

$A(n) = A(n-2) + 2(2)$

$A(n-2) = A(n-3) + 2$

$A(n) = A(n-3) + 2(3)$

$A(n) = A(n-i) + 2i$

$i = n-1$

$A(n) = A(n-n+1) + 2(n-1)$

$A(n) = 2(n-1)$

There are  $2n-2$  additions and subtractions made.

10.  $A(n) + 2A(n-1) - 8A(n-2) = 10$

$A(0) = 0 \quad A(1) = 14$

$A(n) + 2A(n-1) - 8A(n-2) = 0$

$r^2 + 2r - 8 = 0$

$(r-2)(r+4) = 0$

$r_1 = 2 \quad r_2 = -4$

$A(n) = \alpha(2)^n + \beta(-4)^n$

$A(n) = \alpha(2)^n + \beta(-4)^n + 10/4$

$\begin{cases} \alpha \cdot 2^0 + \beta \cdot 0 \cdot (-4)^0 + 10/4 = 0 \\ \alpha \cdot 2^1 + \beta \cdot 1 \cdot (-4)^1 + 10/4 = 14 \end{cases}$

$\begin{cases} \alpha + \beta + 10/4 = 0 \\ 2\alpha - 4\beta + 10/4 = 14 \end{cases}$

$\begin{cases} \alpha + \beta + 10/4 = 0 \\ 2\alpha - 4\beta + 10/4 = 14 \end{cases}$

$s = 6s + 9s = 10$

$4s = 10$

$s = 10/4$

$\alpha = -10/4$

$4\beta = 2\alpha + 10/4$

$4\beta = -10/4$

$\beta = -10/16$

$\beta = -5/8$

$\therefore A(n) = -10/4(2)^n - 5/8(-4)^n$